Improved and fixed various things in type inference

Source/Dafny/DafnyAst.cs
@@ -1913,12 +1913,12 @@ namespace Microsoft.Dafny {
       }
       Contract.Assert(towerA.Count == 1 && towerB.Count == 1);
 
-      if (a.IsBoolType || a.IsCharType || a.IsBigOrdinalType || a.IsTypeParameter || a.IsInternalTypeSynonym || a is TypeProxy) {
-        return a.Equals(b) ? a : null;
-      } else if (a is IntVarietiesSupertype) {
-        return b is IntVarietiesSupertype || b.IsNumericBased(NumericPersuation.Int) || b.IsBitVectorType ? b : null;
+      if (a is IntVarietiesSupertype) {
+        return b is IntVarietiesSupertype || b.IsNumericBased(NumericPersuation.Int) || b.IsBigOrdinalType || b.IsBitVectorType ? b : null;
       } else if (b is IntVarietiesSupertype) {
-        return a.IsNumericBased(NumericPersuation.Int) ? a : null;
+        return a.IsNumericBased(NumericPersuation.Int) || a.IsBigOrdinalType || a.IsBitVectorType ? a : null;
+      } else if (a.IsBoolType || a.IsCharType || a.IsBigOrdinalType || a.IsTypeParameter || a.IsInternalTypeSynonym || a is TypeProxy) {
+        return a.Equals(b) ? a : null;
       } else if (a is RealVarietiesSupertype) {
         return b is RealVarietiesSupertype || b.IsNumericBased(NumericPersuation.Real) ? b : null;
       } else if (b is RealVarietiesSupertype) {
